floyd_ext/DataatSL.v
@@ -27,6 +27,7 @@ Proof.
 Qed.
 
 Lemma disj_data_at: forall sh t1 t2 p1 p2,
+  sepalg.nonunit sh ->
   ~ pointer_range_overlap p1 (sizeof cenv_cs t1) p2 (sizeof cenv_cs t2) ->
   disjointed (EX v: reptype t1, data_at sh t1 v p1) (EX v: reptype t2, data_at sh t2 v p2).
 Proof.
@@ -40,12 +41,13 @@ Proof.
 Qed.
 
 Lemma data_at_conflict: forall sh t1 t2 p1 p2 v1 v2,
+  sepalg.nonunit sh ->
   pointer_range_overlap p1 (sizeof cenv_cs t1) p2 (sizeof cenv_cs t2) ->
   data_at sh t1 v1 p1 * data_at sh t2 v2 p2 |-- FF.
 Proof.
   intros.
   eapply derives_trans; [apply sepcon_derives; apply data_at_memory_block |].
-  apply memory_block_conflict; auto.
+  apply seplog.memory_block_overlap; auto.
 Qed.
 
 End DataAtMSL.
